\documentclass[11pt, a4paper]{article}

\input{preamble}
\input{instructions}

\begin{document}


%%%%%%%%%%%%%%%%%%%%%%%%%%%%%%%%%%%%%%%%%%%%%%%%%%%%
%%%%%%%%%%%%%%%%%%%%   TASK 1   %%%%%%%%%%%%%%%%%%%%
%%%%%%%%%%%%%%%%%%%%%%%%%%%%%%%%%%%%%%%%%%%%%%%%%%%%

% Equation taken from https://arxiv.org/abs/2103.15745
\taskone
    
\begin{task}
%%%%%%%%%%%%%%%%%%%%%%%%%%%%%%%% START EDITING HERE
    \begin{imaths}
        O\left(\frac{x(x-1)}{x^2+1}\right):= &
        \left\langle \frac{x(x-1)}{x^2+1}\right\rangle_{\hskip-4pt 6}\cup
        \left\langle \frac{x(x+1)}{x^2+1}\right\rangle_{\hskip-4pt 6}\cup
        \left\langle \frac{x(x-i)}{x^2-1}\right\rangle_{\hskip-4pt 6}\cup
        \left\langle \frac{x(x+i)}{x^2-1}\right\rangle_{\hskip-4pt 6}\\
        =
        &\left\{\frac{1+x^2}{1-x},\frac{1-x}{1+x^2},\frac{x(x+1)}{x-1},\frac{x(x+1)}{x^2+1},\frac{x^2+1}{x(x+1)},\right.\\
        &\frac{x(1-x)}{x+1},\frac{x+1}{x(1-x)},\frac{x+1}{x^2+1},\frac{x^2+1}{x+1},\frac{x(x-1)}{x^2+1},\frac{x^2+1}{x(x-1)},\\
        &\frac{-ix(x+i)}{x-i},\frac{1-x^2}{i(x-i)},\frac{i(x-i)}{1-x^2},\frac{x(x+i)}{x^2-1},\frac{x^2-1}{x(x+i)},\\
        &\left. \frac{i(x+i)}{x(i-x)},\frac{x(i-x)}{i(x+i)},\frac{i(x+i)}{x^2-1},\frac{x^2-1}{i(x+i)},\frac{x(x-i)}{x^2-1},\frac{x^2-1}{x(x-i)}\right\}.
    \end{imaths}
%%%%%%%%%%%%%%%%%%%%%%%%%%%%%%%% STOP EDITING HERE
\end{task}

\newpage





%%%%%%%%%%%%%%%%%%%%%%%%%%%%%%%%%%%%%%%%%%%%%%%%%%%%
%%%%%%%%%%%%%%%%%%%%   TASK 2   %%%%%%%%%%%%%%%%%%%%
%%%%%%%%%%%%%%%%%%%%%%%%%%%%%%%%%%%%%%%%%%%%%%%%%%%%

% Equation taken from https://arxiv.org/abs/2103.09261
\tasktwo

\begin{task}
%%%%%%%%%%%%%%%%%%%%%%%%%%%%%%%% START EDITING HERE
    \begin{imaths}
       A_{z^m}^*(H_k)(z)&=\sum_{n=0}^\infty \frac{\lambda^n}{\prod_{j=0}^{n-1}(k+j(m-1))}A_{z^m}^*\left(z^{k+n(m-1)}\right)\\
       &=0+\sum_{n=1}^\infty \frac{\lambda^n}{\prod_{j=0}^{n-1}(k+j(m-1))}A_{z^m}^*\left(z^{k+n(m-1)}\right)\\
       &=\sum_{n=1}^\infty \frac{\lambda^n}{\prod_{j=0}^{n-1}(k+j(m-1))}\cdot(k+n(m-1)-m+1)\cdot\left(z^{k+n(m-1)-m+1}\right)\\
       &=\sum_{n=1}^\infty \frac{\lambda^n}{\prod_{j=0}^{n-1}(k+j(m-1))}\cdot(k+(n-1)(m-1))\cdot\left(z^{k+(n-1)(m-1)}\right)\\
        &=\sum_{n=1}^\infty \frac{\lambda\cdot\lambda^{n-1}}{\prod_{j=0}^{n-1}(k+j(m-1))}\left(z^{k+(n-1)(m-1)}\right)\\
        &=\lambda\cdot \sum_{n=0}^\infty \frac{\lambda^n}{\prod_{j=0}^{n-1}(k+j(m-1))}\left(z^{k+n(m-1)}\right)\\
        &=\lambda H_k(z)
    \end{imaths}
%%%%%%%%%%%%%%%%%%%%%%%%%%%%%%%% STOP EDITING HERE
\end{task}

\newpage





%%%%%%%%%%%%%%%%%%%%%%%%%%%%%%%%%%%%%%%%%%%%%%%%%%%%
%%%%%%%%%%%%%%%%%%%%   TASK 3   %%%%%%%%%%%%%%%%%%%%
%%%%%%%%%%%%%%%%%%%%%%%%%%%%%%%%%%%%%%%%%%%%%%%%%%%%

% Equation taken from https://arxiv.org/abs/2103.12163
\taskthree

\begin{task}
\flushleft
%%%%%%%%%%%%%%%%%%%%%%%%%%%%%%%% START EDITING HERE
	Consider the second-order discretized advection equation
	\begin{imaths}
		\dot{q}_n(t) = -c\left(\frac{q_{n-2}(t) - 4 q_{n-1}(t) + 3q_{n}(t)}{2h}\right).\tag{1}
	\end{imaths}
	Following the usual steps, the global relation is
	\begin{imaths}
		 e^{WT} \hat{q}(k,T) - \hat{q}(k,0) - c \left( \frac{ 4 e^{-ikh} f_{0} - e^{-2ikh} f_{0} - e^{-ikh} f_{0} }{2}\right)&= 0, \quad \text{Im}(k) \leq 0,\tag{2}
	\end{imaths}
	with dispersion relation
	\begin{imaths}
		W(k) = c \,\frac{e^{-2ikh} - 4 e^{-ikh} + 3}{2h},\tag{3}
	\end{imaths}
	and nontrivial symmetry
	\begin{imaths}
		\nu_1(k) = \frac{i}{h} \ln\left(4 - e^{-ikh}\right).\tag{4}
	\end{imaths}
	Solving for $\hat{q}(k,T)$ and taking the inverse transform, we obtain
	\begin{imaths}
		q_n(T) &= \frac{1}{2\pi} \int_{-\pi/h}^{\pi/h} e^{iknh} e^{-WT} \hat{q}(k,0)\,dk\tag{5} \\
		&\quad\, + \frac{c}{2\pi} \int_{-\pi/h}^{\pi/h} e^{iknh} e^{-WT} \left( \frac{ 4 e^{-ikh} f_{0} - e^{-2ikh} f_{0} - e^{-ikh} f_{-1} }{2}\right)\,dk.
	\end{imaths}
		With the given Dirichlet boundary condition, we encounter the ghost point $f_{-1}(W,T)$, which is unknown. [\dots] Instead, we return to the continuous problem, where the PDE itself gives the Neumann boundary condition from the Dirichlet condition:
	\begin{imaths}
		q_x(0,t) = \frac{-1}{c}\,q_{t}(0,t) = \frac{-1}{c}\,\frac{\partial}{\partial t} q(0,t) = \frac{-u'(t)}{c} = \frac{-v(t)}{c}, \quad v(t) = u'(t).\tag{6}
	\end{imaths}
%%%%%%%%%%%%%%%%%%%%%%%%%%%%%%%% STOP EDITING HERE
\end{task}


\end{document}